@prefix :        <http://togostanza.org/resource/stanza#> .
@prefix owl:     <http://www.w3.org/2002/07/owl#> .
@prefix rdf:     <http://www.w3.org/1999/02/22-rdf-syntax-ns#> .
@prefix rdfs:    <http://www.w3.org/2000/01/rdf-schema#> .
@prefix spin:    <http://spinrdf.org/spin#> .
@prefix xsd:     <http://www.w3.org/2001/XMLSchema#> .
@prefix dct:     <http://purl.org/dc/terms/> .

<http://togostanza.org/resource/stanza>
      rdf:type          owl:Ontology ;
      dct:license       <http://creativecommons.org/publicdomain/zero/1.0/> ;
      owl:versionInfo   "2015-01-15"^^xsd:date .

# Classes

:Stanza
      rdf:type          owl:Class ;
      rdfs:comment      "A generic class for Stanza." ;
      rdfs:label        "Stanza" ;
      rdfs:subClassOf   owl:Thing ;
      owl:hasKey        (:stanza :label :description :usage :type :context :display :provider :license :parameters) .

:TogoStanza
      rdf:type          owl:Class ;
      rdfs:comment      "A class for TogoStanza." ;
      rdfs:label        "TogoStanza" ;
      rdfs:subClassOf   :Stanza .

:NanoStanza
      rdf:type          owl:Class ;
      rdfs:comment      "A class for NanoStanza." ;
      rdfs:label        "NanoStanza" ;
      rdfs:subClassOf   :Stanza .

:Parameter
      rdf:type          owl:Class ;
      rdfs:comment      "A class for parameters of a Stanza." ;
      rdfs:label        "Parameter" ;
      rdfs:subClassOf   owl:Thing .

:Context
      rdf:type          owl:Class ;
      rdfs:comment      "A generic class for Context describing a context in which the Stanza will be used." ;
      rdfs:label        "Context" ;
      rdfs:subClassOf   owl:Thing .

:GeneContext
      rdf:type          owl:Class ;
      rdfs:comment      "This class is attributed to a Stanza which will be used in a gene context." ;
      rdfs:label        "Gene" ;
      rdfs:subClassOf   :Context .

:OrganismContext
      rdf:type          owl:Class ;
      rdfs:comment      "This class is attributed to a Stanza which will be used in a organism context." ;
      rdfs:label        "Organism" ;
      rdfs:subClassOf   :Context .

:EnvironmentContext
      rdf:type          owl:Class ;
      rdfs:comment      "This class is attributed to a Stanza which will be used in a environment context." ;
      rdfs:label        "Environment" ;
      rdfs:subClassOf   :Context .

:PhenotypeContext
      rdf:type          owl:Class ;
      rdfs:comment      "This class is attributed to a Stanza which will be used in a phenotype context." ;
      rdfs:label        "Phenotype" ;
      rdfs:subClassOf   :Context .

:MediumContext
      rdf:type          owl:Class ;
      rdfs:comment      "This class is attributed to a Stanza which will be used in a medium context." ;
      rdfs:label        "Medium" ;
      rdfs:subClassOf   :Context .

:OtherContext
      rdf:type          owl:Class ;
      rdfs:comment      "This class is attributed to a Stanza which will be used in a other context." ;
      rdfs:label        "Other" ;
      rdfs:subClassOf   :Context ;
      owl:disjointWith  :GeneContext, :OrganismContext, :EnvironmentContext, :PhenotypeContext, :MediumContext .

:Display
      rdf:type          owl:Class ;
      rdfs:comment      "A generic class for Display indicating visual style used in the Stanza." ;
      rdfs:label        "Display" ;
      rdfs:subClassOf   owl:Thing .

:TableDisplay
      rdf:type          owl:Class ;
      rdfs:comment      "This class is used to indicate the Stanza has a table style representation." ;
      rdfs:label        "Table" ;
      rdfs:subClassOf   :Display .

:ChartDisplay
      rdf:type          owl:Class ;
      rdfs:comment      "This class is used to indicate the Stanza has a chart style representation." ;
      rdfs:label        "Chart" ;
      rdfs:subClassOf   :Display .

:TreeDisplay
      rdf:type          owl:Class ;
      rdfs:comment      "This class is used to indicate the Stanza has a tree style representation." ;
      rdfs:label        "Tree" ;
      rdfs:subClassOf   :Display .

:GraphDisplay
      rdf:type          owl:Class ;
      rdfs:comment      "This class is used to indicate the Stanza has a graph style representation." ;
      rdfs:label        "Graph" ;
      rdfs:subClassOf   :Display .

:MapDisplay
      rdf:type          owl:Class ;
      rdfs:comment      "This class is used to indicate the Stanza has a map style representation." ;
      rdfs:label        "Map" ;
      rdfs:subClassOf   :Display .

:TextDisplay
      rdf:type          owl:Class ;
      rdfs:comment      "This class is used to indicate the Stanza has a text style representation." ;
      rdfs:label        "Text" ;
      rdfs:subClassOf   :Display .

:ImageDisplay
      rdf:type          owl:Class ;
      rdfs:comment      "This class is used to indicate the Stanza has a image style representation." ;
      rdfs:label        "Image" ;
      rdfs:subClassOf   :Display .

:OtherDisplay
      rdf:type          owl:Class ;
      rdfs:comment      "This class is used to indicate the Stanza has an other style representation." ;
      rdfs:label        "Other" ;
      rdfs:subClassOf   :Display .

# Properties for Stanza

:stanza
      rdf:type          owl:DatatypeProperty ;
      rdf:comment       "This property specifies a name of the Stanza." ;
      rdfs:domain       :Stanza ;
      rdfs:range        xsd:string .

:label
      rdf:type          owl:DatatypeProperty ;
      rdf:comment       "This property specifies a display name of the Stanza." ;
      rdfs:domain       :Stanza ;
      rdfs:range        xsd:string ;
      rdfs:subPropertyOf rdfs:label .

:description
      rdf:type          owl:DatatypeProperty ;
      rdf:comment       "This property is used to describe the Stanza." ;
      rdfs:domain       :Stanza ;
      rdfs:range        xsd:string ;
      rdfs:subPropertyOf rdfs:comment .

:usage
      rdf:type          owl:DatatypeProperty ;
      rdf:comment       "This property is used to show how to embed in a Web page." ;
      rdfs:domain       :Stanza ;
      rdfs:range        xsd:string .

:type
      rdf:type          owl:ObjectProperty ;
      rdf:comment       "This property is used to specify a type of the Stanza." ;
      rdfs:domain       :Stanza ;
      rdfs:range        [ rdf:type owl:Class; owl:unionOf (:TogoStanza :NanoStanza) ] .

:context
      rdf:type          owl:ObjectProperty ;
      rdf:comment       "This property describes in which context the Stanza will be used"; 
      rdfs:domain       :Stanza ;
      rdfs:range        [ rdf:type owl:Class; owl:unionOf (:GeneContext :OrganismContext :EnvironmentContext :PhenotypeContext :MediumContext) ] .

:display
      rdf:type          owl:ObjectProperty ;
      rdf:comment       "This propoerty describes in which visual style the Stanza will be displayed" ;
      rdfs:domain       :Stanza ;
      rdfs:range        [ rdf:type owl:Class; owl:unionOf (:TableDisplay :ChartDisplay :TreeDisplay :GraphDisplay :MapDisplay :TextDisplay :ImageDisplay :OtherDisplay) ] .

:provider
      rdf:type          owl:DatatypeProperty ;
      rdf:comment       "This property is used to indicate a name of the service provider of the Stanza." ;
      rdfs:domain       :Stanza ;
      rdfs:range        xsd:string .

:license
      rdf:type          owl:ObjectProperty ;
      rdf:comment       "This property is used to specify a license of the Stanza." ;
      rdfs:domain       :Stanza ;
      rdfs:range        rdfs:Resource .

:author
      rdf:type          owl:DatatypeProperty ;
      rdf:comment       "This property is used to indicate a name of the developer of the Stanza." ;
      rdfs:domain       :Stanza ;
      rdfs:range        xsd:string .

:address
      rdf:type          owl:DatatypeProperty ;
      rdf:comment       "This property is used to indicate a e-mail address of the developer of the Stanza." ;
      rdfs:domain       :Stanza ;
      rdfs:range        xsd:string .

:created
      rdf:type          owl:DatatypeProperty ;
      rdf:comment       "This property is used to indicate a initial creation date of the Stanza." ;
      rdfs:domain       :Stanza ;
      rdfs:range        xsd:date .

:updated
      rdf:type          owl:DatatypeProperty ;
      rdf:comment       "This property is used to indicate a updated date of the Stanza." ;
      rdfs:domain       :Stanza ;
      rdfs:range        xsd:date .

:parameters
      rdf:type          owl:ObjectProperty ;
      rdf:comment       "This property is used to link with a blank node which has a set of parameters for the Stanza." ;
      rdfs:domain       :Stanza ;
      rdfs:range        :Parameter .

# Properties for parameters

:key
      rdf:type          owl:DatatypeProperty ;
      rdf:comment       "This property is used to indicate a name of the parameter variable." ;
      rdfs:domain       :Parameter ;
      rdfs:range        xsd:string .

:example
      rdf:type          owl:DatatypeProperty ;
      rdf:comment       "This property is used to indicate an example of the parameter value." ;
      rdfs:domain       :Parameter ;
      rdfs:range        xsd:string .

:description
      rdf:type          owl:DatatypeProperty ;
      rdf:comment       "This property is used to describe the parameter." ;
      rdfs:domain       :Parameter ;
      rdfs:range        xsd:string .

:required
      rdf:type          owl:DatatypeProperty ;
      rdf:comment       "This property is used to indicate if the parameter is mandatory or not." ;
      rdfs:domain       :Parameter ;
      rdfs:range        xsd:boolean .

